Added explicit instantiation for FMUs

simplefmi/SimpleFMI.thy
@@ -1,20 +1,31 @@
 theory SimpleFMI
-  imports "../theories/utp_time_rel"
+  imports 
+    "../theories/utp_time_rel"
+    "../theories/utp_reactive_hoare"
+    "../hybrid/utp_hybrid"    
 begin
 
 purge_notation Sublist.parallel (infixl "\<parallel>" 50)
     
-type_synonym '\<alpha> fmu = "'\<alpha> trel"
+record '\<alpha> fmu =
+  fmi2Instantiate :: "'\<alpha> trel"
+  fmi2DoStep      :: "'\<alpha> trel"
+
 type_synonym '\<alpha> ma = "'\<alpha> trel"
   
 definition fmu_single ("FMU[_, _]") where
-[upred_defs]: "fmu_single a P = rel_aext P (map_st\<^sub>L a)"
+[upred_defs]: "fmu_single a fmu = 
+  \<lparr> fmi2Instantiate = rel_aext (fmi2Instantiate fmu) (map_st\<^sub>L a)
+  , fmi2DoStep = rel_aext (fmi2Instantiate fmu) (map_st\<^sub>L a) \<rparr>"
 
-definition fmu_comp :: "'\<alpha> fmu \<Rightarrow> '\<alpha> fmu \<Rightarrow> '\<alpha> fmu" (infixr "\<parallel>" 85) where
+definition fmu_comp :: "'\<alpha> trel \<Rightarrow> '\<alpha> trel \<Rightarrow> '\<alpha> trel" (infixr "\<parallel>" 85) where
 [upred_defs]: "fmu_comp P Q = (P \<and> Q)"
   
 definition FMI :: "('\<alpha> \<Rightarrow> '\<alpha>) \<Rightarrow> '\<alpha> fmu list \<Rightarrow> '\<alpha> trel \<Rightarrow> ('\<alpha> \<Rightarrow> '\<alpha>) \<Rightarrow> '\<alpha> trel" where
-[upred_defs]: "FMI Init FMUs MA Wiring = \<langle>Init\<rangle>\<^sub>r ;; (((foldr fmu_comp FMUs true) \<parallel> MA) ;; \<langle>Wiring\<rangle>\<^sub>r)\<^sup>\<star>"
+[upred_defs]: "FMI Init FMUs MA Wiring = 
+                 (foldr fmu_comp (map fmi2Instantiate FMUs) true) ;;  
+                 \<langle>Init\<rangle>\<^sub>r ;; 
+                 (((foldr fmu_comp (map fmi2DoStep FMUs) true) \<parallel> MA) ;; \<langle>Wiring\<rangle>\<^sub>r)\<^sup>\<star>"
 
 definition ArbStep :: "'\<alpha> ma" where
 [upred_defs]: "ArbStep = true"
@@ -29,5 +40,30 @@ lemma fmu_comp_true [simp]:
 lemma fmu_comp_ArbStep [simp]: 
   "P \<parallel> ArbStep = P"
   by (rel_auto)
+    
+(*
+lemma fmu_hoare_rp [hoare_safe]:
+  "\<lbrakk> x \<natural> p; \<lbrace>p\<restriction>\<^sub>px\<rbrace>Q\<lbrace>p\<restriction>\<^sub>px\<rbrace>\<^sub>r \<rbrakk> \<Longrightarrow> \<lbrace>p\<rbrace>FMU[x, Q]\<lbrace>p\<rbrace>\<^sub>r"
+  apply (rel_simp, auto simp add: des_vars.defs rp_vars.defs)
+  apply (rename_tac ok wait tr st ok' wait' tr' st')
+  apply (drule_tac x="ok" in spec)
+  apply (drule_tac x="wait" in spec)
+  apply (drule_tac x="tr" in spec)
+  apply (drule_tac x="get\<^bsub>x\<^esub> st" in spec)
+  apply (drule_tac x="ok'" in spec)
+  apply (drule_tac x="wait'" in spec)
+  apply (drule_tac x="tr'" in spec)
+  apply (drule_tac x="get\<^bsub>x\<^esub> st'" in spec)
+  apply (auto)
+done
+
+lemma fmi_hoare_rp:
+  assumes "\<lbrace>true\<rbrace>\<langle>Init\<rangle>\<^sub>r ;; \<langle>Wiring\<rangle>\<^sub>r\<lbrace>p\<rbrace>\<^sub>r" "\<And> fmu. fmu \<in> set(FMUs) \<Longrightarrow> \<lbrace>p\<rbrace>\<langle>Wiring\<rangle>\<^sub>r ;; fmu\<lbrace>p\<rbrace>\<^sub>r"
+  shows "\<lbrace>true\<rbrace>FMI Init FMUs MA Wiring\<lbrace>p\<rbrace>\<^sub>r"
+oops
+*)  
+    
+definition Modelica_FMU :: "(unit, '\<alpha>::t2_space) hyrel \<Rightarrow> '\<alpha> fmu" where
+[upred_defs]: "Modelica_FMU P = \<lparr> fmi2Instantiate = II\<^sub>r, fmi2DoStep = H2T(P) \<rparr>"
     
 end
